process.v
@@ -78,96 +78,22 @@ Definition sta_swi (I O : Ty) (b : bool) (p : Proc I O) :=
                     (p)
   )))).
 
-Definition process_pool
-  (n : nat)
-  (f_coopt : nat -> bool)
-  (f_initial : nat -> bool)
-  (f_I f_O : nat -> Ty)  
-  (T' : Ty)
-  (f_proj : [T'] -> forall n, [Option (f_I n)])
-  (f_proc : forall n, Proc (f_I n) (f_O n)) : Proc (Times Nat T') (times_on n f_O).
-  elim: n.
-  - simpl.
-    eapply map. simpl.
-    instantiate (1:= Times Bool (Option (f_I 0))). exact (fun i => (i.1 == 0, f_proj i.2 0)). 
-    exact id.  
-    apply swi. exact (f_initial 0). 
-    apply maybe. 
-    eapply map.
-      eapply id. 
-      exact (fun o => (f_coopt 0,o)).
-    exact (f_proc 0).
 
-  - intros. rewrite /times_on. simpl.
-    apply par.
-    * eapply map.
-      instantiate (1:= Times Bool (Option (f_I n.+1))). simpl.
-      exact (fun i => (i.1 == n.+1,f_proj i.2 n.+1)).
-        exact id. 
-      eapply swi.
-        exact (f_initial n.+1). 
-      eapply maybe.
-      eapply map.
-        exact id.     
-        exact (fun o => (f_coopt n.+1,o)).
-      (*eapply maybe.*) (*not necessary anymore*)
-        exact (f_proc n.+1).
-        apply H.
-Defined.
 
 Definition inr_or_def {A B : Set} (def: B) (x : A + B) := if x is inr x' then x' else def.
 
-Definition loop_and_count
-  (stateType : Ty)           
-  (state : [stateType])
-  (T_in T_out T' : Ty)                
-  (f_I : [Sum T_in T_out] -> [stateType] -> [stateType])
-  (def : [T_out])
-  (p : Proc (Times Nat T') T_out)
-  (f_si : [Times stateType (Sum T_in T_out)] -> [Option (Times Nat T')])
-  : Proc T_in T_out :=
-  (@map T_in (Sum T_in T_out) (Sum T_in T_out) T_out inl (inr_or_def def)
-                          (@loop (Sum T_in T_out)
-                             (@map _ _ (Times _ _) _
-                                id snd
-                                (@sta _ _ stateType f_I (fun _ v => v) state
-                                   (@map (Times stateType (Sum _ _ ))
-                                      (Option (Times Nat T')) _ (Sum T_in T_out) f_si inr (maybe p)))))).
-
-(*Definition loop_and_count
-  (stateType : Ty)           
-  (state : [stateType])
-  (T_in' T_out' : Ty)                
-  (f_I : [Sum T_in' T_out'] -> [stateType] -> [stateType])
-  (def : [T_out'])
-  (p : Proc (Times Nat T_in') T_out')
-  (f_si : [Times stateType (Sum T_in' T_out')] -> [Option (Times Nat T_in')])
-  : Proc T_in' T_out' :=
-  (@map T_in' (Sum T_in' T_out') (Sum T_in' T_out') T_out' inl (inr_or_def def)
-                          (@loop (Sum T_in' T_out')
-                             (@map _ _ (Times _ _) _
-                                id snd
-                                (@sta _ _ stateType f_I (fun _ v => v) state
-                                   (@map (Times stateType (Sum _ _ ))
-                                      (Option (Times Nat T_in')) _ (Sum T_in' T_out') f_si inr (maybe p)))))).*)
-(*maybe p eliminates input, since we only want it for state change
- very cool, this still wroks for bad example too because we will switch to disk handler after next output
- This is similar to cpu cycle where we check the ic at the end of the cycle.*)
-
-
-(*Example*)
 
 Definition mask := Bool.
 Definition pending := Bool.
 Definition I_bits := Times pending mask.
-Definition ic := Times I_bits (Times I_bits I_bits). (*new definition*)
+Definition ic := Times I_bits (Times I_bits I_bits).
 Definition count := Nat.
 Definition re_sch := Bool.
 Definition prev_pid := Option Nat.
-Definition cur_pid := Nat.
+Definition cur_pid := Sum Bool Nat. (*false = defaultInterrupt, true=diskInterrupt*)
+(*Definition pids := Times cur_pid prev_pid.*)
 Definition pids := Times cur_pid prev_pid.
 Definition bool_state := Times re_sch ic.
-(* I_list removed: all interrupts are always present *)
 Definition all_interrupts : seq [TInterrupt] :=
   [:: TimerInterrupt; DiskInterrupt; DefaultInterrupt].
 Definition stateType := Times pids bool_state.
@@ -181,7 +107,7 @@ Definition get_ic (v : [stateType]) := (get_bool_state v).2.
 
 Definition get_I_bits' (ic : [ic]) (ir : [TInterrupt]) : [I_bits] :=
   match ir with
-  | DefaultInterrupt   => ic.1
+  | DefaultInterrupt => ic.1  (*default pending is always true*)
   | DiskInterrupt    => ic.2.1
   | TimerInterrupt => ic.2.2
   end.
@@ -201,7 +127,7 @@ Definition update_re_sch (v : [stateType]) re_sch : [stateType] := update_bool_s
 
 Definition update_I_bits' (myic : [ic]) (ir : [TInterrupt]) (bits : [I_bits]) : [ic] :=
   match ir with
-  | DefaultInterrupt  => (bits, myic.2)
+  | DefaultInterrupt => (bits, myic.2)         (* keep only the mask; discard pending *)
   | DiskInterrupt    => (myic.1, (bits, myic.2.2))
   | TimerInterrupt => (myic.1, (myic.2.1, bits))
   end.
@@ -216,7 +142,7 @@ Definition update_I_mask (v : [stateType]) (ir : [TInterrupt ]) mask : [stateTyp
 
 Definition or_I_bits (b1 b2 : [I_bits]) : [I_bits] := (b1.1 || b2.1, b1.2 || b2.2).
 Definition or_ic (c1 c2 : [ic]) : [ic] :=
-  (or_I_bits c1.1 c2.1,
+  (or_I_bits c1.1  c2.1,
    (or_I_bits c1.2.1 c2.2.1,
     or_I_bits c1.2.2 c2.2.2)).
 Definition or_bool_state (s1 s2 : [bool_state]) : [bool_state] := (s1.1 || s2.1, or_ic s1.2 s2.2).
@@ -228,86 +154,20 @@ Definition unset_masks (v : [stateType]) : [stateType] :=
 Definition masks_set (v : [stateType]) :=
   foldr (fun I b => (get_I_mask v I) && b) true all_interrupts.
 
+Definition my_f_I := fun (n : nat) => if n == 4 then THandlerOutput else if n == 3 then Empty else  Unit.
 
-(*Definition mask := Bool.
-Definition pending := Bool.
-Definition I_bits := Times pending mask.
-(*Definition ic := Arrow TInterrupt I_bits.*)
-Definition ic := Times I_bits (Times I_bits I_bits).
-Definition count := Nat.
-Definition re_sch := Bool.
-Definition prev_pid := Option Nat.
-Definition cur_pid := Nat.
-Definition pids := Times cur_pid prev_pid.
-(*Definition stateType := Times (Times cur_pid re_sch) ic.*)
-Definition bool_state := Times re_sch ic.
-Definition I_list := List TInterrupt.
-Definition stateType := Times pids (Times I_list bool_state).
+(*Definition I_output_type := Times THandlerOutput bool_state.*)
 
-(*Definition get_count (v : [stateType]) := v.1.1.*)
-Definition get_pids (v : [stateType]) := v.1.
-Definition get_I_list (v : [stateType]) := v.2.1.
-Definition get_bool_state (v : [stateType]) := v.2.2.
-Definition get_cur_pid (v : [stateType]) := (get_pids v).1.
-Definition get_prev_pid (v : [stateType]) := (get_pids v).2.
-Definition get_re_sch (v : [stateType]) := (get_bool_state v).1.
-Definition get_ic (v : [stateType]) := (get_bool_state v).2.
-Definition get_I_bits' (ic : [ic]) (ir : [TInterrupt]) : [I_bits] := ic ir. 
-Definition get_I_bits (v : [stateType]) (ir : [TInterrupt]) := get_I_bits' (get_ic v) ir.
-
-Definition get_pending' (bits : [I_bits]) := bits.1.
-Definition get_mask' (bits : [I_bits]) := bits.2.
-
-Definition get_I_pending (v : [stateType]) (ir : [TInterrupt]) := get_pending' (get_I_bits v ir).
-Definition get_I_mask (v : [stateType]) (ir : [TInterrupt]) := get_mask' (get_I_bits v ir).
-
-Definition update_pids (v : [stateType]) pids : [stateType] := (pids,v.2).
-Definition update_I_list (v : [stateType]) l : [stateType] := (v.1,(l,v.2.2)).
-Definition update_bool_state (v : [stateType]) bs : [stateType] := (v.1,(v.2.1,bs)).
-Definition update_cur_pid (v : [stateType]) cur_pid : [stateType] := update_pids v (cur_pid,(get_pids v).2).
-Definition update_prev_pid (v : [stateType]) prev_pid : [stateType] := update_pids v ((get_pids v).1,prev_pid).
-Definition update_re_sch (v : [stateType]) re_sch : [stateType] := update_bool_state v (re_sch,(get_bool_state v).2).
-Definition update_I_bits' (myic : [ic])  (ir : [TInterrupt]) (bits : [I_bits]) : [ic] := fun (i : [TInterrupt]) => if i == ir then bits else myic i.
-
-Definition update_ic (v : [stateType]) ic : [stateType] := update_bool_state v ((get_bool_state v).1,ic).
-Definition update_I_bits (v : [stateType]) (ir : [TInterrupt]) (bits : [I_bits]) := update_ic v (update_I_bits' (get_ic v) ir bits).
-
-Definition update_I_pending (v : [stateType]) (ir : [TInterrupt]) pending : [stateType] :=
-  update_I_bits v ir (pending,get_I_mask v ir).
-Definition update_I_mask (v : [stateType]) (ir : [TInterrupt ]) mask : [stateType] :=
-  update_I_bits v ir (get_I_pending v ir,mask).
-
-Definition or_I_bits (b1 b2 : [I_bits]) : [I_bits] := (b1.1 || b2.1, b1.2 || b2.2).
-Definition or_ic (c1 c2 : [ic]) : [ic] := fun (i : [TInterrupt]) => or_I_bits (c1 i) (c2 i).
-Definition or_bool_state (s1 s2 : [bool_state]) : [bool_state] := (s1.1 || s2.1, or_ic s1.2 s2.2).
+Definition my_f_O := fun (n : nat) => if n == 3 then Nat else if n == 4 then TTypeSyscall else if n == 5 then TPublicOutput else (Times THandlerOutput Bool).
 
 
-Definition set_masks (v : [stateType]) : [stateType] := foldr (fun I v' => update_I_mask v' I true) v (get_I_list v).
-Definition unset_masks (v : [stateType]) : [stateType] := foldr (fun I v' => if I \in get_I_list v then update_I_mask v' I false else v') v (get_I_list v).
-Definition masks_set (v : [stateType]) := foldr (fun I b => (get_I_mask v I) && b) true (get_I_list v).
-*)
-
-
-Definition my_f_I := fun (n : nat) => if n == 4 then THandlerOutput else Unit.
-
-Definition I_output_type := Times THandlerOutput bool_state.
-
-Definition my_f_O := fun (n : nat) => if n == 3 then Nat else if n == 4 then TTypeSyscall else if n == 5 then TPublicOutput else I_output_type.
-
-
-Definition T_in := Sum TInterrupt Unit.
-Definition T_out' := Times (Option TPublicOutput) (Times (Option TTypeSyscall) (Times (Option Nat) (times_on 2 (fun _ => I_output_type)))).
+Definition T_in := TInterrupt.
+Definition T_out' := Times (Option TPublicOutput) (Times (Option TTypeSyscall) (Times (Option Nat) (times_on 2 (fun _ => Times THandlerOutput Bool)))).
 Definition T' := Option THandlerOutput.
 Definition is_sch_out (o : [T_out']) :=
   match o with
   | (None,(None,(Some n,_))) => Some n
   | _ => None                                   
-  end.
-
-Definition is_I_in (i : [T_in]) :=
-  match i with
-  | inl ir => Some ir
-  | inr _ => None
   end.
 
 (*Definition all_interrupts : seq [TInterrupt] := [::TimerInterrupt;DiskInterrupt].*)
@@ -328,21 +188,31 @@ Definition default_I_out (o : [T_out']) :=
   | (_,(_,(_,(x,(_,_))))) => x
   end.  
 
-Definition is_I_out_done (o : [T_out']) : [Option (Times TInterrupt bool_state)] :=
+Definition is_I_out_done (o : [T_out']) : [Option (Times TInterrupt Bool)] :=
   if tI_out o is Some (Notify,b) then Some (TimerInterrupt,b)
   else if dI_out o is Some (Notify,b) then Some (DiskInterrupt,b)
   else if default_I_out o is Some (Notify,b) then Some (DefaultInterrupt,b)
   else None.          
 
 
-Definition is_user_pid (p : [cur_pid]) : bool := (3 < p).
-Definition is_sch (p : [cur_pid]) : bool := p == 3.
-Definition handler_pid := 3.
-Definition is_handler_pid (p : [cur_pid]) : bool := p == handler_pid.
+Definition is_user_pid (p : [cur_pid]) : bool := if p is inr _ then true else false.
+Definition is_sch (p : [cur_pid]) : bool := p == inr 1.
+Definition scheduler_pid : [cur_pid] := inr 1.
 
-(* interrupt handlers live at pids 3 (timer) and 4 (disk) *)
+(*we distinguish disk and default interrupt handler because their output is secret*)
+Definition nat_to_cur_pid (n : nat) : [cur_pid ] :=
+  match n with
+  | 0 => inr 0 (*timer interrupt*)
+  | 1 => inl true (*disk interrupt*)
+  | 2 => inl false (*default interrupt*)
+  | 3 => inr 1 (*scheduler*)
+  | 4 => inr 2 (*high p*)
+  | 5 => inr 3 (*low p*)
+  | n => inr n             
+  end.
+             
 Definition I_handler_pid (ir : [TInterrupt]) : [cur_pid] :=
-  index ir all_interrupts.
+  nat_to_cur_pid (index ir all_interrupts).
 
 (* a handler is selectable iff pending and not masked *)
 Definition I_ready (v : [stateType]) (ir : [TInterrupt]) : bool :=
@@ -352,28 +222,119 @@ Definition first_ready (v : [stateType]) : option [TInterrupt] :=
   ohead [seq ir <-  all_interrupts | (I_ready v ir) ].
 
 (* before overriding cur_pid, save it to prev_pid if it is a user process *)
+
+(*Definition update_prev_pid_wrap (v : [stateType]) (n : [cur_pid]) : [stateType] :=
+  if n is inr n' then update_prev_pid v (Some n') else v.*)
+
 Definition save_cur_to_prev (v : [stateType]) : [stateType] :=
-  if is_user_pid (get_cur_pid v)
-  then update_prev_pid v (Some (get_cur_pid v))
+  if get_cur_pid v is inr n
+  then update_prev_pid v (Some n)
   else v.
 
 
-(*
-output scenarios
-- a handler finishes
-- a handler running, not finished
-- scheduler choice
-- public/private output
+Definition false_I_bits : [I_bits] := (false,false).
+Definition false_ic : [ic] := ((false,false),(false_I_bits,false_I_bits)).
+Definition bad_to_bs (ir : [TInterrupt]) (b : [Bool]) : [bool_state] :=
+  match ir with
+    | TimerInterrupt => (true,false_ic)
+    | DiskInterrupt => (false,false_ic)
+  | DefaultInterrupt => (false,false_ic)
+  end.
 
- *)
+(*Definition step_on_input (i : [T_in]) (v : [stateType]) : [stateType] :=*)
+ 
 
-(*issues*)
-Definition f_I (i : [Sum T_in T_out']) (v : [stateType]) : [stateType] :=
+Definition check_scheduler (o : [T_out']) (v : [stateType])  :=
+  if @is_sch_out o is Some n then update_cur_pid v (inr n) else v.
+
+Definition check_handlers (to_bs : [TInterrupt] -> [Bool] -> [bool_state]) (o : [T_out']) (v : [stateType])  :=
+  if is_I_out_done o is Some (ir,b) then
+    update_bool_state v (or_bool_state (get_bool_state (unset_masks v)) (to_bs ir b)) else v.
+
+Definition initiate_handler (ir : [TInterrupt]) (v : [stateType]) :=
+  update_I_pending (set_masks (update_cur_pid (save_cur_to_prev v) (I_handler_pid ir))) ir false.
+
+Definition initiate_scheduler  (v : [stateType]) := update_re_sch (update_prev_pid (update_cur_pid v scheduler_pid) None) false.
+
+Definition get_prev_pid_wrap (v : [stateType]) : [Option cur_pid] := if get_prev_pid v is Some n then Some (inr n) else None.
+Definition initiate_prev_pid  (v : [stateType]) := update_prev_pid (update_cur_pid v (odflt scheduler_pid (get_prev_pid_wrap v))) None.
+
+Definition inspect_output (to_bs : [TInterrupt] -> [Bool] -> [bool_state]) (o : [T_out']) : [stateType] -> [stateType] :=
+  (check_handlers to_bs o) \o check_scheduler o.
+
+Definition compute_next_pid (o : [T_out']) (v : [stateType]) : [stateType] :=
+  match first_ready v with
+  | Some ir => initiate_handler ir v 
+  | None => if is_I_out_done o is None then v
+            else if (get_re_sch v)
+                 then initiate_scheduler v
+                 else initiate_prev_pid v
+  end.
+
+Definition step_on_output (to_bs : [TInterrupt] -> [Bool] -> [bool_state]) (o : [T_out']) : [stateType] -> [stateType]:=
+  (compute_next_pid o) \o (inspect_output to_bs o).
+
+
+
+Lemma sta_comp : forall (I V O : Ty) (IRel : myrel [I]) (VRel : myrel [V]) (ORel : myrel [O]) (f f' : [I] -> [V] -> [V]) (g : [O] -> [V] -> [V])
+                        (v : [V]) (p : Proc (Times V I) O),
+    fv_NI ORel VRel VRel g ->
+    fv_NI IRel VRel VRel f -> f_EP IRel VRel f ->
+    fv_NI IRel VRel VRel f' -> f_EP IRel VRel f' ->
+    NI (eqpair_R VRel IRel) ORel p ->    
+    NI IRel (eqpair VRel ORel) (sta (fun i => (f i) \o (f' i)) g v p).
+Proof.
+  intros.
+  apply sta_NI;eauto.
+  move: H0 H2. clear.
+  rewrite /fv_NI. intros. eauto.
+  move: H1 H3. clear.
+  rewrite /f_EP. intros. eauto.
+Qed.
+
+Definition step_left (f : [T_in] -> [stateType] -> [stateType]) : [Sum T_in T_out'] -> [stateType] -> [stateType] :=
+  fun i v => 
   match i with
-  | inl i => if is_I_in i is Some ir then update_I_pending v ir true else v
+  | inl i => f i v
+  | inr _ => v
+  end.
+
+Definition step_right (f : [T_out'] -> [stateType] -> [stateType]) : [Sum T_in T_out'] -> [stateType] -> [stateType] :=
+  fun i v => 
+  match i with
+  | inl _ => v
+  | inr o => f o v
+  end.
+
+Definition initiate_next :  [T_out'] -> [stateType] -> [stateType] := fun o v =>  if first_ready v is Some ir then
+                                                                                             initiate_handler ir v
+                                                                                           else if is_I_out_done o is Some _ then
+                                                                                                  if get_re_sch v then initiate_scheduler v else initiate_prev_pid v
+                                                                                                else v.
+                                                                                                  
+                                                                                                                 
+(*Definition maybe_initiate_scheduler :  [T_out'] -> [stateType] -> [stateType] := fun o v => if first_ready v is Some _ then v else if is_I_out_done o is None then v else if get_re_sch v then initiate_scheduler v else v.
+Definition maybe_initiate_prev_pid : [T_out'] -> [stateType] -> [stateType] := fun o v => if first_ready v is Some _ then v else if is_I_out_done o is None then v else if ~~ get_re_sch v then initiate_prev_pid v else v.*)
+Definition step0 := step_left (fun i v => update_I_pending v i true).
+Definition step1 := step_right check_scheduler.
+Definition step2  (to_bs : [TInterrupt] -> [Bool] -> [bool_state]) := step_right (check_handlers to_bs).
+Definition step3 := step_right initiate_next.
+(*Definition step4 := step_right maybe_initiate_scheduler.
+Definition step5 := step_right maybe_initiate_prev_pid.*)
+
+
+Definition state_step (to_bs : [TInterrupt] -> [Bool] -> [bool_state]) (i : [Sum T_in T_out']) : [stateType] -> [stateType] :=
+  (step3 i) \o (step2 to_bs i) \o (step1 i) \o (step0 i).
+
+
+
+
+(*Definition f_I (to_bs : [TInterrupt] -> [Bool] -> [bool_state]) (i : [Sum T_in T_out']) (v : [stateType]) : [stateType] :=
+  match i with
+  | inl i => 
   | inr o => let v := if @is_sch_out o is Some n then update_cur_pid v n else v in (*apply scheduler choice, lowest priority*)
-             let v:= if is_I_out_done o is Some (ir,bstate) then
-                         update_bool_state v (or_bool_state (get_bool_state (unset_masks v)) bstate) else v in
+             let v:= if is_I_out_done o is Some (ir,b) then
+                         update_bool_state v (or_bool_state (get_bool_state (unset_masks v)) (to_bs ir b)) else v in
              match first_ready v with
              | Some ir => (update_I_pending (set_masks (update_cur_pid (save_cur_to_prev v) (I_handler_pid ir))) ir false)
              | None => if is_I_out_done o is None then v
@@ -381,62 +342,56 @@ Definition f_I (i : [Sum T_in T_out']) (v : [stateType]) : [stateType] :=
                             then update_re_sch (update_prev_pid (update_cur_pid v handler_pid) None) false
                             else update_prev_pid (update_cur_pid v (odflt handler_pid (get_prev_pid v))) None
              end
-  end.
+  end.*)
 
 (*We only reroute disk interrupts*)
 Definition is_I_out (o : [T_out']) : [Option THandlerOutput] :=
-  if dI_out o is Some (o',_) then Some o' else None.
-(*  
-  if tI_out o is Some (o',_) then Some o'
-  else if dI_out o is Some (o',_) then Some o'
-  else if default_I_out o is Some (o',b) then Some o'
+if dI_out o is Some (o',_) then Some o'
        else None.
-*)
 
-Definition f_si (si : [Times stateType (Sum T_in T_out')]) : [Option (Times Nat T')] :=
-  if si.2 is inr o then Some (get_cur_pid si.1, @is_I_out o) else None.
+(*discards input from the inner process, only allowed to affect bit in ic, not pid*)
+Definition f_si (si : [Times stateType (Sum T_in T_out')]) : [Option (Times cur_pid T')] :=
+  if si.2 is inr o then Some (get_cur_pid si.1, is_I_out o) else None.
 
 Definition low_p := @out Unit TPublicOutput GetRequest.
 Definition high_p := @alternate_generic2 THandlerOutput TTypeSyscall Unit1 Syscall NOP tt (fun i => i == Notify).
 
-Definition handler_type := Proc Unit I_output_type.
-Definition false_I_bits : [I_bits] := (false,false).
-Definition false_ic : [ic] := (false_I_bits,(false_I_bits,false_I_bits)).
+Definition handler_type := Proc Unit (Times THandlerOutput Bool).
 
-Definition I_handler (b: [bool_state]) : handler_type.
+Definition I_handler : handler_type.
   rewrite /handler_type.
   eapply map. exact id.
   instantiate (1:= Times Nat Unit).
-  exact (fun o => if o.1 == 0 then (Notify,b) else (Nothing,(false,false_ic))).
+  exact (fun o => if o.1 == 0 then (Notify,false) else (Nothing,false)).
   eapply sta. exact (fun _ v => v). exact (fun _ v => v.+1%%2).
   exact 0.
   apply out. exact tt.
 Defined.
 
-Definition bad_tI_handler : handler_type := I_handler (true,false_ic).
-Definition bad_dI_handler : handler_type := I_handler (false,false_ic).
-Definition bad_default_handler : handler_type := I_handler (false,false_ic).
+(*Definition bad_tI_handler : handler_type := I_handler. (*false_ic all of them*) (*re_sch = true only for timer interrupt handler*)
+Definition bad_dI_handler : handler_type := I_handler.
+Definition bad_default_handler : handler_type := I_handler.*)
 
-Definition scheduler : Proc Unit Nat.
+Definition scheduler : Proc Empty Nat.
   eapply map. exact id.
-  instantiate (1:= Times Nat Unit). exact (fun o => fst o + 4). (*skip first three processes to reach high_p (0) and low_p (1) *)
+  instantiate (1:= Times Nat Unit). exact (fun o => fst o + 2). (*skip first three processes to reach high_p (0) and low_p (1) *)
   eapply sta. exact (fun _ v => v). exact (fun _ v => v.+1%%2).
   exact 1. (*Will start scheduling high process*)
   apply out. exact tt.
 Defined.
 
+(*the only way handlers differ in what flags they set. This has been moved out of the handler itself and is interpreted from the Notify output
+   they give. For example Notify from timer interrupt implies re_sch should be set to true. *)
 Definition my_procs_bad : forall n, Proc (my_f_I n) (my_f_O n).
-  case. apply bad_tI_handler.
-  case. apply bad_dI_handler.
-  case. apply bad_default_handler.
+  case. apply I_handler. (*timer interrupt handler*)
+  case. apply I_handler. (*disk interrupt handler*)
+  case. apply I_handler. (*default handler*)
   case. cbv. apply scheduler.
   case. apply high_p.  
   case. apply low_p.
-  elim. apply bad_default_handler.
-  intros. apply bad_default_handler.
+  elim. apply I_handler.
+  intros. apply I_handler.
 Defined.
-
-Print T'.
 
 Definition f_proj (i : [T']) : forall n, [Option (my_f_I n)].
   simpl. rewrite /my_f_I. intros. case_if.
@@ -444,20 +399,92 @@ Definition f_proj (i : [T']) : forall n, [Option (my_f_I n)].
   exact None. 
 Defined.
 
+
+Definition process_pool
+  (n : nat)
+  (f_coopt : nat -> bool)
+  (f_initial : nat -> bool)
+  (f_I f_O : nat -> Ty)  
+  (T' : Ty)
+  (f_proj : [T'] -> forall n, [(Option (f_I n))])
+  (f_pid : [cur_pid] -> [Nat])
+  (f_proc : forall n, Proc (f_I n) (f_O n)) : Proc (Times cur_pid T') (times_on n f_O).
+  elim: n.
+  - simpl.
+    eapply map. simpl.
+    instantiate (1:= Times Bool (Option (f_I 0))). exact (fun i => (f_pid i.1 == 0, f_proj i.2 0)). 
+    exact id.  
+    apply swi. exact (f_initial 0). 
+    apply maybe. 
+    eapply map.
+      eapply id. 
+      exact (fun o => (f_coopt 0,o)).
+    exact (f_proc 0).
+
+  - intros. rewrite /times_on. simpl.
+    apply par.
+    * eapply map.
+      instantiate (1:= Times Bool (Option (f_I n.+1))). simpl.
+      exact (fun i => (f_pid i.1 == n.+1,f_proj i.2 n.+1)).
+        exact id. 
+      eapply swi.
+        exact (f_initial n.+1). 
+      eapply maybe.
+      eapply map.
+        exact id.     
+        exact (fun o => (f_coopt n.+1,o)).
+      (*eapply maybe.*) (*not necessary anymore*)
+        exact (f_proc n.+1).
+        apply H.
+Defined.
+
 Definition my_f_coopt (n : nat) : bool := true.
-Definition initial_pid := 5. (*starting with low process*)
-Definition my_f_initial (n : nat) := n == initial_pid.
-Definition my_process_pool_bad := @process_pool 5 my_f_coopt my_f_initial my_f_I my_f_O T' f_proj my_procs_bad.
-Definition initial_state_bad : [stateType] := ((initial_pid,None),(false,false_ic)).
+Definition initial_pid : [cur_pid] := inr 3. (*starting with low process*)
+
+Definition my_f_pid (pid : [cur_pid]) : [Nat] :=
+  match pid with
+  | inl true => 1 (*disk interrupt*)
+  | inl false => 2 (*default interrupt*)
+  | inr 0 => 0
+  | inr 1 => 3
+  | inr 2 => 4
+  | inr 3 => 5
+  | inr n => n             
+  end.
+
+Definition my_f_initial (n : nat) := n == (my_f_pid initial_pid).
+
+
+
+Definition my_process_pool_bad := @process_pool 5 my_f_coopt my_f_initial my_f_I my_f_O T' f_proj my_f_pid my_procs_bad.
+Definition initial_state : [stateType] := ((initial_pid,None),(false,false_ic)).
 Definition def : [ T_out' ]  := (None,(None,(None,(None,(None,None))))).
 
-Definition model_bad : Proc T_in T_out' := @loop_and_count stateType initial_state_bad T_in T_out' T' f_I def my_process_pool_bad f_si.
+
+Definition loop_sta
+  (stateType : Ty)           
+  (state : [stateType])
+  (T_in T_out T' : Ty)                
+  (f_I : [Sum T_in T_out] -> [stateType] -> [stateType])
+  (def : [T_out])
+  (p : Proc (Times cur_pid T') T_out)
+  (f_si : [Times stateType (Sum T_in T_out)] -> [Option (Times cur_pid T')])
+  : Proc T_in T_out :=
+  (@map T_in (Sum T_in T_out) (Sum T_in T_out) T_out inl (inr_or_def def)
+                          (@loop (Sum T_in T_out)
+                             (@map _ _ (Times _ _) _
+                                id snd
+                                (@sta _ _ stateType f_I (fun _ v => v) state
+                                   (@map (Times stateType (Sum _ _ ))
+                                      (Option (Times cur_pid T')) _ (Sum T_in T_out) f_si inr (maybe p)))))).
+
+
+Definition model_bad : Proc T_in T_out' := @loop_sta stateType initial_state T_in T_out' T' (state_step bad_to_bs) def my_process_pool_bad f_si.
 
 Definition Tsum' := ([T_in] + [T_out'])%type.
 
-Definition inr_tt : Tsum' := inl (inr tt).
-Definition dI' : Tsum' := inl (inl DiskInterrupt).
-Definition tI' : Tsum' := inl (inl TimerInterrupt). 
+Definition dI' : Tsum' := inl DiskInterrupt.
+Definition tI' : Tsum' := inl TimerInterrupt. 
 Definition low_out x : [T_out'] := (Some x,(None,(None,(None,(None,None))))).
 Definition high_out x : [T_out'] := (None,(Some x,(None,(None,(None,None))))).
 Definition sch_o x : [T_out'] := (None,(None,(Some x,(None,(None,None))))).
@@ -465,18 +492,18 @@ Definition defaultI_o x : [T_out'] := (None,(None,(None,(Some x,(None,None))))).
 Definition dI_o x : [T_out'] := (None,(None,(None,(None,(Some x,None))))).
 Definition tI_o x : [T_out'] := (None,(None,(None,(None,(None,Some x))))).
 
-Definition tI_yes' : Tsum' :=  inr (tI_o (Notify,(true,false_ic))).
-Definition tI_no' : Tsum' :=  inr (tI_o (Nothing,(false,false_ic))).
+Definition tI_yes' : Tsum' :=  inr (tI_o (Notify,false)).
+Definition tI_no' : Tsum' :=  inr (tI_o (Nothing,false)).
 
-Definition dI_yes' : Tsum' :=  inr (dI_o (Notify,(false,false_ic))).
-Definition dI_no' : Tsum' :=  inr (dI_o (Nothing,(false,false_ic))).
+Definition dI_yes' : Tsum' :=  inr (dI_o (Notify,false)).
+Definition dI_no' : Tsum' :=  inr (dI_o (Nothing,false)).
 
 Definition pub_get' : Tsum' := inr (low_out GetRequest).
 Definition pr_nop' : Tsum' := inr (high_out NOP).
 Definition pr_sys' : Tsum' := inr (high_out Syscall).
 
-Definition sch_low : Tsum' := inr (sch_o 5).
-Definition sch_high : Tsum' := inr (sch_o 4).
+Definition sch_low : Tsum' := inr (sch_o 3).
+Definition sch_high : Tsum' := inr (sch_o 2).
 
 Definition seqtype' := seq Tsum'.
 Eval cbv in T_out'.
@@ -488,20 +515,75 @@ Definition with_dI' : seqtype' := [::pub_get';dI';pub_get';dI_no';dI_yes';pub_ge
 (*Definition output_rel' := eqpair (eqmaybe (publicRel TPublicOutput)) (eqpair (eqmaybe (semiprivateRel TTypeSyscall)) (eqmaybe (semiprivateRel THandlerOutput))).*)
 (*Definition output_rel := eqmaybe (eqsum_R (publicRel TPublicOutput) (semiprivateRel TTypeSyscall)).*)
 
-Ltac rewr := rewrite /model_bad /loop_and_count /my_process_pool_bad /process_pool /my_f_initial /low_p /my_f_coopt /alternate_generic /alternate_generic2 /high_p /f_si /tI_o /bad_tI_handler /I_handler /f_proj /scheduler /bad_dI_handler /is_I_out /bad_default_handler /low_out.
+Ltac rewr := rewrite /model_bad /loop_sta /my_process_pool_bad /process_pool /my_f_initial /low_p /my_f_coopt /alternate_generic /alternate_generic2 /high_p /f_si /tI_o /I_handler /f_proj /scheduler /low_out /is_I_out.
 
 Ltac lsolv := try solve [ reduce_tac;reduce_tac | reduce_tac;try solve [reduce_once | econ];simpl;first (reduce_tac;reduce_tac)];simpl.
 Ltac reduce_tac2 :=
   (try rewr);
    (repeat
       reduce_once);(try swi_instans); rewrite ?eqxx /= /xor /=.
+
+
+(* Concrete handler pids, so `reduce_state` never has to reduce TInterrupt's
+   deriving-generated equality (index ir all_interrupts) — which is flaky under
+   simpl/cbn. reflexivity (full conversion) discharges these fine. *)
+(*Lemma I_handler_pid_timer   : I_handler_pid TimerInterrupt   = 0. Proof. reflexivity. Qed.
+Lemma I_handler_pid_disk    : I_handler_pid DiskInterrupt    = 1. Proof. reflexivity. Qed.
+Lemma I_handler_pid_default : I_handler_pid DefaultInterrupt = 2. Proof. reflexivity. Qed.*)
+
+(* Unfolding lemmas: since we hide these below with `Opaque`, `unfold`/`simpl` no
+   longer expose their bodies. Use `rewrite f_I_eq` (etc.) to unfold on demand. Each
+   RHS is the definition's own body, captured with `cbv delta`, so nothing is copied
+   by hand and the lemmas stay in sync with the definitions automatically. Stated
+   here while the constants are still transparent, so `reflexivity` closes them. *)
+Lemma f_I_eq : state_step = ltac:(let x := eval cbv delta [state_step] in state_step in exact x).
+Proof. reflexivity. Qed.
+Lemma f_si_eq : f_si = ltac:(let x := eval cbv delta [f_si] in f_si in exact x).
+Proof. reflexivity. Qed.
+Lemma initial_state_bad_eq :
+  initial_state = ltac:(let x := eval cbv delta [initial_state] in initial_state in exact x).
+Proof. reflexivity. Qed.
+Lemma def_eq : def = ltac:(let x := eval cbv delta [def] in def in exact x).
+Proof. reflexivity. Qed.
+Lemma f_proj_eq : f_proj = ltac:(let x := eval cbv delta [f_proj] in f_proj in exact x).
+Proof. reflexivity. Qed.
+
+(* Collapse a tower of state getters/updaters into the concrete value it computes.
+   Unfolds the base (initial_state_bad is Opaque) via its eq-lemma, replaces the
+   handler-pid indices with their literals, delta-reduces only the state layer with
+   cbv (so no eqType/other constants get dragged in), and finishes booleans/nats
+   with simpl. Over a concrete base this yields a ground tuple; over an abstract
+   state v it collapses to a tuple of expressions in v's fields. *)
+(*Ltac reduce_state :=
+  rewrite ?initial_state_bad_eq
+          (*?I_handler_pid_timer ?I_handler_pid_disk ?I_handler_pid_default*);
+  cbv [ state_step step0 step1 step2 step3 step4 step5 step_left step_right (*maybe_initiate_prev_pid maybe_initiate_scheduler maybe_initiate_handler*) get_pids get_bool_state get_cur_pid get_prev_pid get_re_sch get_ic
+        get_I_bits get_I_bits' get_pending' get_mask' get_I_pending get_I_mask
+        update_pids update_bool_state update_cur_pid update_prev_pid update_re_sch
+        update_ic update_I_bits update_I_bits' update_I_pending update_I_mask
+        or_I_bits or_ic or_bool_state
+        set_masks unset_masks all_interrupts save_cur_to_prev is_user_pid
+        (*default_on_ic*) false_ic false_I_bits initial_pid (*check_handlers initiate_handler initiate_scheduler*)
+        compute_next_pid inspect_output
+        foldr fst snd ];
+  simpl.*)
+
+
+Ltac sta_state_reduce :=
+  match goal with
+  | |- context [(@sta (Sum T_in T_out') (Sum T_in T_out') stateType (state_step _) _ ?state _)] =>let reduced := eval cbv in state in
+                                                                                                          pattern state; match goal with |- ?F state => change (F reduced) end; cbv beta
+  end.                                                                                                             
+
 Lemma trace_no_dI' : forall l, Trace (publicRel _) l no_dI' model_bad.
 Proof.  
   intros.
   rewr;simpl;rewr;simpl;rewr;simpl;rewr.
 
-  do 12(first [econ;[idtac | econ | idtac] | econ];
-        reduce_tac;try solve [reflexivity| reduce_tac;reduce_tac];simpl;try swi_instans).
+  sta_state_reduce.
+
+   do 12 (first [econ;[idtac | econ | idtac] | econ];
+         reduce_tac;try solve [reflexivity| reduce_tac;reduce_tac];simpl;try swi_instans;sta_state_reduce).
 
   (*proved the last element of the trace manually to avoid evar holes in proof*)
    (first [econ;[idtac | econ | idtac] | econ];
@@ -517,7 +599,7 @@ Proof.
   rewr;simpl;rewr;simpl;rewr;simpl;rewr.
 
   do 17(first [econ;[idtac | econ | idtac] | econ];
-        reduce_tac;try solve [reflexivity| reduce_tac;reduce_tac];simpl;try swi_instans).
+        reduce_tac;try solve [reflexivity| reduce_tac;reduce_tac];simpl;try swi_instans;sta_state_reduce).
 
   (*proved the last element of the trace manually to avoid evar holes in proof*)  
    (first [econ;[idtac | econ | idtac] | econ];
@@ -527,9 +609,9 @@ Proof.
    econ. reduce_tac. econ. econ. reduce_tac. econ.
 Qed.   
 
-Definition good_ic := ((false,true),((false,true),(false,false))).
+(*Definition good_ic := ((false,((false,false),(false,false))).*)
 
-Definition initial_state_good : [stateType] := ((initial_pid,None),(false,good_ic)).
+(*Definition initial_state_good : [stateType] := ((initial_pid,None),(false,good_ic)).*)
 
 Definition T'_good := Times (Option THandlerOutput) Bool.
 
@@ -538,24 +620,51 @@ Definition to_T'_good (o : [T_out']) : [T'_good] :=
   let o' := if dI_out o is Some (o',_) then Some o' else None in
   (o',b).
 
-Definition my_f_I_good := fun (n : nat) => if n == 0 then Unit else if n == 4 then THandlerOutput else if n < 3 then Bool else Unit.
+Definition my_f_I_good (n : nat) :=
+  match n with
+  | 0 => Unit (*tI*)
+  | 1 => Bool (*dI*)
+  | 2 => Bool (*defaultI*)
+  | 3 => Empty (*scheduler*)         
+  | 4 => THandlerOutput (*high*)
+  | 5 => Unit (*low*)
+  | _ => Unit (*padding*)           
+  end.
+
+Definition my_f_O_good (n : nat) :=
+  match n with
+  | 0 => Times THandlerOutput Bool (*tI*)
+  | 1 => Times THandlerOutput Bool (*dI*)
+  | 2 => Times THandlerOutput Bool (*defaultI*)
+  | 3 => Nat (*scheduler*)         
+  | 4 => TTypeSyscall (*high*)
+  | 5 => TPublicOutput (*low*)
+  | _ => Unit (*padding*)           
+  end.
+                    
+(*                            if n == 0 then Unit else if n == 4 then THandlerOutput else if n < 3 then Bool else Unit.*)
+(*Definition my_f_O_good := fun (n : nat) => if n == 0 then THandlerOutput else if n == 3 then Nat else if n == 4 then TTypeSyscall else if n == 5 then TPublicOutput else Times THandlerOutput Bool.*)
 
 
-    
+
 (*We extend the input to schedulers so we can distinguish if the latest output was Notify by timer interrupt.
  This will feed their counter.
  true = from finishing timer interrupt, reset counter
  false = output pulse, decrement counter*)
 Definition f_proj_good (i : [T'_good]) : forall n, [Option (my_f_I_good n)].
   simpl. rewrite /my_f_I_good. intros.
-  case_if. exact None. (*timer interrupt handler does not need any information*)
-  case_if.
-  exact (fst i).
-  case_if. exact (Some (snd i)). (*other interrupts receive bool, true -> timer interrupt just finished, set count = 2, false -> decrement counter*)
-  exact None.
+  case: n. exact None. (*timer interrupt handler does not need any information*)
+  case. exact (Some (snd i)). (*dI gets tick*)
+  case. exact (Some (snd i)). (*defaultI gets tick*)
+  case. exact None. (*scheduler receives nothing*)
+  case. exact (fst i). (*high process receives dI outut*)
+  case. exact None. (*low process receives nothing*)
+  move=>_. exact None.
 Defined.  
+(*other interrupts receive bool, true -> timer interrupt just finished, set count = 2, false -> decrement counter*)
 
-Definition good_handler_type := Proc Bool I_output_type.
+
+Definition good_handler_type := Proc Bool (Times THandlerOutput Bool).
 Definition default_on_ic : [ic] := ((true,false),((false,false),(false,false))). (*pending set for default*)
 Definition mask_most : [ic] := ((false,true),((false,true),(false,false))). (*mask set for everything but timer interrupt*)
 
@@ -567,36 +676,43 @@ Definition mask_most : [ic] := ((false,true),((false,true),(false,false))). (*ma
  All handlers take 2 units of time to complete, so by enforcing a time slice equal to length of a handler we never stop handlers mid execution.
  Assuming all handlers take the same amount of time and that we don't interrupt mid handling, are simplifying assumptions.
  *)
-Definition good_I_handler (n : nat) (b : [bool_state]) : good_handler_type.
+Definition good_I_handler (n : nat) : good_handler_type.
   eapply map. exact id.
   2: eapply sta.
   instantiate (2:= Nat).
-  instantiate (1:= I_output_type).
-  exact (fun o => if o.1 != 0 then o.2 else (o.2.1,or_bool_state o.2.2 (false,mask_most))). (*in the else case, o.2.1 will always be Notify and o.2.2 will be b*)
-  exact (fun b n' => if b then n else n').
-  exact (fun o n' => n'.-1).
+  instantiate (1:= THandlerOutput).
+  exact (fun o => if o.1 != 0 then (o.2,false) else (o.2,true)).
+  exact (fun b n' => if b then n else n'.-1).
+  exact (fun o n' => n').
   exact n.
-  eapply map. instantiate (1:= Unit). exact (fun i => tt). exact id.
-  apply (I_handler b).
+  eapply map.
+  instantiate (1:= Unit). exact (fun i => tt).
+  instantiate (1:= Times THandlerOutput _). exact fst.
+  apply I_handler.
 Defined.
 
-Definition time_slice := 2. 
-Definition good_tI_handler : handler_type := I_handler (true,default_on_ic).
-Definition good_dI_handler : good_handler_type := good_I_handler time_slice (false,default_on_ic).
-Definition good_default_handler : good_handler_type := good_I_handler time_slice (false,default_on_ic).      
+Definition time_slice := 3. 
+Definition good_tI_handler : handler_type := I_handler.
+Definition good_dI_handler : good_handler_type := good_I_handler time_slice.
+Definition good_default_handler : good_handler_type := good_I_handler time_slice.
 
-Definition my_good_procs : forall n, Proc (@my_f_I_good n) (my_f_O n).
+Definition unit_proc : Proc Unit Unit.
+  apply out. exact tt.
+Defined.
+
+
+Definition my_good_procs : forall n, Proc (@my_f_I_good n) (my_f_O_good n).
   case. apply good_tI_handler.
   case. apply good_dI_handler.
   case. apply good_default_handler.
   case. apply scheduler.
   case. apply high_p.
   case. apply low_p.
-  elim. apply bad_default_handler.
-  intros. apply bad_default_handler.
+  elim. apply unit_proc.
+  intros. apply unit_proc.
 Defined.
 
-Definition my_process_pool_good := @process_pool 5 my_f_coopt my_f_initial my_f_I_good my_f_O T'_good f_proj_good my_good_procs.
+Definition my_process_pool_good := @process_pool 5 my_f_coopt my_f_initial my_f_I_good my_f_O_good T'_good f_proj_good my_f_pid my_good_procs.
 
 Definition def_good : [ T_out' ]  := (None,(None,(None,(None,(None,None))))).
 
@@ -610,42 +726,66 @@ Definition def_good : [ T_out' ]  := (None,(None,(None,(None,(None,None))))).
   case. case=>h. intros. exact (Some (h,true)). exact None.
 Defined.*)
 
-Definition f_si_good (si : [Times stateType (Sum T_in T_out')]) : [Option (Times Nat T'_good)] :=
+Definition f_si_good (si : [Times stateType (Sum T_in T_out')]) : [Option (Times cur_pid T'_good)] :=
   if si.2 is inr o then Some (get_cur_pid si.1, to_T'_good o) else None.
 
-Definition model_good := @loop_and_count stateType initial_state_good T_in T_out' T'_good f_I def_good my_process_pool_good f_si_good.
-Print model_bad.
-Print model_good.
+Definition good_to_bs (ir : [TInterrupt]) (b : [Bool]) : [bool_state] :=
+  let ic := ((true,b),((false,b),(false,false))) in
+  match ir with
+    | TimerInterrupt => (true,ic)
+    | DiskInterrupt => (false,ic)
+  | DefaultInterrupt => (false,ic)
+  end.    
 
 
-Definition tI_no'g : Tsum' :=  inr (tI_o (Nothing,(false,false_ic))).
-Definition tI_yes'g : Tsum' :=  inr (tI_o (Notify,(true,default_on_ic))).
+Definition initial_state_good : [stateType] := ((initial_pid,None),(false,mask_most)).
 
-Definition default_and_masked_ic := or_bool_state (false, default_on_ic) (false, mask_most).
+Definition model_good := @loop_sta stateType initial_state_good T_in T_out' T'_good (state_step good_to_bs) def_good my_process_pool_good f_si_good.
 
-Definition dI_no'g : Tsum' :=  inr (dI_o (Nothing,(false,false_ic))).
-Definition dI_yes'g : Tsum' :=  inr (dI_o (Notify,default_and_masked_ic)).
 
+Definition tI_no'g : Tsum' :=  inr (tI_o (Nothing,false)).
+Definition tI_yes'g : Tsum' :=  inr (tI_o (Notify,false)).
+
+(*Definition default_and_masked_ic := or_bool_state (false, default_on_ic) (false, mask_most).*)
+
+Definition dI_no'g : Tsum' :=  inr (dI_o (Nothing,false)).
+Definition dI_yes'g : Tsum' :=  inr (dI_o (Notify,false)).
+Definition dI_terminate'g : Tsum' :=  inr (dI_o (Notify,true)).
 
                                      
-Definition defaultI_no'g : Tsum' :=  inr (defaultI_o (Nothing,(false,false_ic))).
-Definition defaultI_yes'g : Tsum' :=  inr (defaultI_o (Notify,default_and_masked_ic)).
+Definition defaultI_no'g : Tsum' :=  inr (defaultI_o (Nothing,false)).
+Definition defaultI_yes'g : Tsum' :=  inr (defaultI_o (Notify,false)).
+Definition defaultI_terminate'g : Tsum' :=  inr (defaultI_o (Notify,true)).
 
-Definition good_no_dI' : seqtype' :=   [::pub_get';                      tI';pub_get';tI_no'g;tI_yes'g;defaultI_no'g;defaultI_yes'g;sch_high;pr_nop'(*nop*);tI';pr_nop';tI_no'g;tI_yes'g;defaultI_no'g;defaultI_yes'g;sch_low;pub_get'].
-Definition good_with_dI' : seqtype' := [::pub_get';dI';pub_get';pub_get';tI';pub_get';tI_no'g;tI_yes'g;dI_no'g;dI_yes'g;sch_high;pr_sys'(*sys*);tI';pr_nop';tI_no'g;tI_yes'g;defaultI_no'g;defaultI_yes'g;sch_low;pub_get'].
-
-
-Ltac rewr ::= rewrite /model_bad /loop_and_count /my_process_pool_bad /process_pool /my_f_initial /low_p /my_f_coopt /alternate_generic /alternate_generic2 /high_p /f_si /tI_o /bad_tI_handler /I_handler /f_proj /scheduler /bad_dI_handler /is_I_out /bad_default_handler /low_out /model_good /my_process_pool_good /f_si_good /to_T'_good /f_proj_good /good_default_handler /good_tI_handler /good_dI_handler /good_I_handler.
+Definition good_no_dI' : seqtype' :=   [::pub_get';                      tI';pub_get';tI_no'g;tI_yes'g;defaultI_no'g;defaultI_yes'g;defaultI_no'g;defaultI_terminate'g;sch_high;pr_nop'(*nop*);tI';pr_nop';tI_no'g;tI_yes'g;defaultI_no'g;defaultI_yes'g;defaultI_no'g;defaultI_terminate'g;sch_low;pub_get'].
+Definition good_with_dI' : seqtype' := [::pub_get';dI';pub_get';pub_get';tI';pub_get';tI_no'g;tI_yes'g;dI_no'g      ;dI_yes'g      ;defaultI_no'g;defaultI_terminate'g;sch_high;pr_sys'(*sys*);tI';pr_nop';tI_no'g;tI_yes'g;defaultI_no'g;defaultI_yes'g;defaultI_no'g;defaultI_terminate'g;sch_low;pub_get'].
 
 
+Ltac rewr ::= rewrite /model_bad /loop_sta /my_process_pool_bad /process_pool /my_f_initial /low_p /my_f_coopt /alternate_generic /alternate_generic2 /high_p /f_si /tI_o /I_handler /f_proj /scheduler /is_I_out /low_out /model_good /my_process_pool_good /f_si_good /to_T'_good /f_proj_good /good_default_handler /good_tI_handler /good_dI_handler /good_I_handler.
 
+
+(*Ltac reduce_state' :=
+  rewrite ?initial_state_bad_eq
+          (*?I_handler_pid_timer ?I_handler_pid_disk ?I_handler_pid_default*);
+  cbv [ state_step step_on_input step_on_output get_pids get_bool_state get_cur_pid get_prev_pid get_re_sch get_ic
+        get_I_bits get_I_bits' get_pending' get_mask' get_I_pending get_I_mask
+        update_pids update_bool_state update_cur_pid update_prev_pid update_re_sch
+        update_ic update_I_bits update_I_bits' update_I_pending update_I_mask
+        or_I_bits or_ic or_bool_state
+        set_masks unset_masks all_interrupts save_cur_to_prev is_user_pid
+        (*default_on_ic*) false_ic false_I_bits initial_pid check_handlers initiate_handler initiate_scheduler check_scheduler I_handler_pid
+        foldr fst snd ];
+  simpl.*)
+(*
+(inr 0, Some 3, (false, (true, (false, true, (false, true)))))
+ *)
 Lemma trace_good_no_dI' : forall l, Trace (publicRel _) l good_no_dI' model_good.
 Proof.  
   intros.
   rewr;simpl;rewr;simpl;rewr;simpl;rewr.
 
-  do 16(first [econ;[idtac | econ | idtac] | econ];
-        reduce_tac;try solve [reflexivity| reduce_tac;reduce_tac];simpl;try swi_instans).
+  do 20(first [econ;[idtac | econ | idtac] | econ];
+        reduce_tac;try solve [reflexivity| reduce_tac;reduce_tac];simpl;try swi_instans;sta_state_reduce).
 
    (first [econ;[idtac | econ | idtac] | econ];
     reduce_tac2;try solve [reflexivity| reduce_tac2;reduce_tac2];simpl;try swi_instans).
@@ -659,8 +799,8 @@ Proof.
   intros.
   rewr;simpl;rewr;simpl;rewr;simpl;rewr.
 
-  do 19(first [econ;[idtac | econ | idtac] | econ];
-        reduce_tac;try solve [reflexivity| reduce_tac;reduce_tac];simpl;try swi_instans).
+  do 23(first [econ;[idtac | econ | idtac] | econ];
+        reduce_tac;try solve [reflexivity| reduce_tac;reduce_tac];simpl;try swi_instans;sta_state_reduce).
 
    (first [econ;[idtac | econ | idtac] | econ];
     reduce_tac2;try solve [reflexivity| reduce_tac2;reduce_tac2];simpl;try swi_instans).
@@ -691,14 +831,14 @@ Definition TInterrupt_rel : myrel [TInterrupt].
 Defined.  
 
 
-Definition in_rel : myrel [T_in] := eqsum_L TInterrupt_rel (publicRel _).
-Eval cbv in T_out'.
+Definition in_rel : myrel [T_in] := TInterrupt_rel.
+
 Definition out_rel : myrel [T_out'] := eqpair (eqmaybe (publicRel _))
                                           (eqpair (eqmaybe (semiprivateRel _))
                                              (eqpair (eqmaybe (publicRel _))
-                                                (eqpair (eqmaybe (publicRel _))
+                                                (eqpair (eqmaybe_top (semiprivateRel _))
                                                    (eqpair (eqmaybe_top (semiprivateRel _))
-                                                      (eqmaybe_top (semiprivateRel _)))))).
+                                                      (eqmaybe (publicRel _)))))).
 
 Lemma Trace_imp : forall (A B : Ty) (p : Proc A B) (s : seq ([A] + [B])) l (BRel BRel' : myrel [B]), (forall x y, rel BRel l x y -> rel BRel' l x y) -> Trace BRel l s p -> Trace BRel' l s p.
 Proof.  
@@ -727,22 +867,7 @@ Proof.
   eapply Trace_imp. 2:eapply helper_trace'.
   intros. simpl in H. subst. auto.
 Qed.  
-(* Unfolding lemmas: since we hide these below with `Opaque`, `unfold`/`simpl` no
-   longer expose their bodies. Use `rewrite f_I_eq` (etc.) to unfold on demand. Each
-   RHS is the definition's own body, captured with `cbv delta`, so nothing is copied
-   by hand and the lemmas stay in sync with the definitions automatically. Stated
-   here while the constants are still transparent, so `reflexivity` closes them. *)
-Lemma f_I_eq : f_I = ltac:(let x := eval cbv delta [f_I] in f_I in exact x).
-Proof. reflexivity. Qed.
-Lemma f_si_eq : f_si = ltac:(let x := eval cbv delta [f_si] in f_si in exact x).
-Proof. reflexivity. Qed.
-Lemma initial_state_bad_eq :
-  initial_state_bad = ltac:(let x := eval cbv delta [initial_state_bad] in initial_state_bad in exact x).
-Proof. reflexivity. Qed.
-Lemma def_eq : def = ltac:(let x := eval cbv delta [def] in def in exact x).
-Proof. reflexivity. Qed.
-Lemma f_proj_eq : f_proj = ltac:(let x := eval cbv delta [f_proj] in f_proj in exact x).
-Proof. reflexivity. Qed.
+
 
 (* Part B (see plan): keep the large *data* leaves folded during this proof so
    coq-lsp does not serialize their unfolded bodies while `match_dd` inverts the
@@ -750,15 +875,14 @@ Proof. reflexivity. Qed.
    inversion, so hiding them cannot block `match_dd`. NOTE: my_f_I/my_f_O (type
    indices) and my_f_initial (feeds the swi bool that reduce_swiO/swiO2 must see
    concretely) are deliberately NOT hidden. Scoped to this lemma; restored below. *)
-Opaque f_I f_si initial_state_bad def f_proj.
-
+Opaque state_step f_si initial_state def f_proj.
 
 Lemma model_bad_not_NI : ~ NI in_rel out_rel model_bad.
 Proof.
   intro. rewrite /NI in H. move: (H false). clear H.
   rewrite /NI_l. case=>_ [] + _. intros.
   move: helper_trace.
-  move/a. move/(_ (inl DiskInterrupt) 0). simpl.
+  move/a. move/(_ (DiskInterrupt) 0). simpl.
   have: ir_dis false DiskInterrupt. ssa.
   move=>aa. move/(_ aa).
   move=>Htr. clear a aa.
@@ -769,7 +893,7 @@ Proof.
   move: H9. clear. simpl. ssa.
 Qed.
 
-Transparent f_I f_si initial_state_bad def f_proj.
+Transparent f_si initial_state def f_proj.
 
 Lemma test_test l i i' : rel (eqsum_L in_rel out_rel) l i i' -> is_inl i /\ is_inl i' \/ is_inr i /\ is_inr i'.
 Proof.
@@ -831,9 +955,9 @@ Proof.
   move=>/eqmaybe_public_not_bot=>->//.
   move=>/eqmaybe_semiprivate_not_bot'=>->//.
   move=>/eqmaybe_public_not_bot=>->//.
+  move=>/eqmaybe_semiprivate_not_bot=>->//.
+  move=>/eqmaybe_semiprivate_not_bot=>->//.  
   move=>/eqmaybe_public_not_bot=>->//.
-  move=>/eqmaybe_semiprivate_not_bot=>->//.
-  move=>/eqmaybe_semiprivate_not_bot=>->//.
 Qed.
 
 Lemma falseRel_aware : forall l, aware falseRel true l.
@@ -841,7 +965,7 @@ Proof.
 intros. rewrite /aware. intros. ssa. subst. simpl. intro. ssa.
 Qed.
 
-Definition lt_dis (nP : nat -> Prop) (l : level) (n : nat) := nP n /\ l = \bot.
+(*Definition lt_dis (nP : nat -> Prop) (l : level) (n : nat) := nP n /\ l = \bot.
 
 Definition natLTRel (nP : nat -> Prop) : myrel ([Nat]).
   refine (@MyRel _
@@ -860,8 +984,33 @@ Definition natLTRel (nP : nat -> Prop) : myrel ([Nat]).
   rewrite /order lex0 in H. move/eqP : H=>->. done.
   ssa. move: H. rewrite /lt_dis. ssa. subst.
   con. intros. ssa. ssa. de H0. subst. done.
-Defined.
-(*nP = {1,2} (disk or default handler)*)
+Defined.*)
+
+Print stateType. Print pids. Print cur_pid. Print bool_state.
+Print ic.
+Definition pids_rel : myrel [pids] := eqpair (eqsum (semiprivateRel _) (publicRel _)) (publicRel _).
+Definition hidden_pending : myrel [I_bits] := eqpair (semiprivateRel _) (publicRel _).
+Definition public_pending : myrel [I_bits] := eqpair (publicRel _) (publicRel _).
+Definition ic_rel : myrel [ic] := eqpair hidden_pending (eqpair hidden_pending public_pending).
+Definition bool_state_rel : myrel [bool_state] := eqpair (publicRel _) ic_rel.
+Definition stateType_rel : myrel [stateType] := eqpair pids_rel bool_state_rel.
+Check state_step.
+Transparent state_step f_si initial_state def f_proj.
+Lemma state_step_inl i v : state_step good_to_bs (inl i) v = update_I_pending v i true.
+Proof. reflexivity. Qed.
+
+Lemma in_rel_eq i i0 l : rel in_rel l i i0 -> i = i0.
+Proof.
+  ssa. de H. move: H H0. rewrite /ir_dis. ssa. subst. done.
+Qed.
+
+
+Lemma fv_NI_comp : forall (I O V: Ty) (IRel : myrel [I]) (VRel : myrel [V]) (f f' : [I]  -> [V] ->  [V]),
+    fv_NI IRel VRel VRel f -> fv_NI IRel VRel VRel f' -> fv_NI IRel VRel VRel (fun i => (f' i) \o (f i)).
+Proof.
+intros. move: H H0. rewrite /fv_NI. ssa.
+Qed.
+
 Lemma model_good_NI : NI in_rel out_rel model_good.
 Proof.
   rewr;simpl;rewr;simpl.
@@ -878,134 +1027,178 @@ Proof.
   eauto. eauto.
   mrw. intros.
   2:apply sta_NI. apply rel_eqpair in H. destruct H. eauto.
-  instantiate (1:= eqpair (eqpair (natLTRel 2) (semiprivateRel _)) (semiprivateRel _)). ssa. mrw. intros.
-  simpl in H0. subst.
+  instantiate (1:= stateType_rel). ssa.
+
+
+  
+
+
+  mrw. intros. (*instantiate stateType_rel here*)
+
+
   apply test_test in H as H'.
-  destruct H'. destruct i. destruct i'. ssa.
-  destruct i. destruct i0. destruct H. subst. ssa. ssa.
-  rewrite /ir_dis in H H2. ssa. subst. done. done. de i0. ssa. ssa.
-  destruct i. ssa. destruct i'. ssa.
-  apply rel_eqsum_L2' in H. Print T_out'. Print I_output_type.
-  apply out_rel_not_bot in H. subst. eauto. done.
-  subst. eauto.
+  destruct H'.
+  destruct i;try solve [(exfalso;ssa)].
+  destruct i';try solve [(exfalso;ssa)].  
+  rewrite !state_step_inl.
+  apply rel_eqsum_L' in H. apply in_rel_eq in H. subst.
+  move: H0. clear. 
+  move/rel_eqpair=>[H0] /rel_eqpair[H1] /rel_eqpair[]/rel_eqpair[H2 H3] /rel_eqpair[]/rel_eqpair[H4 H5] /rel_eqpair[] H6 H7.
 
-  mrw. intros. destruct i. 2:ssa.
-  have: dis in_rel l i. ssa. clear H=>H.
-  destruct (eqVneq l \bot). subst. ssa.
-  ssa. de i. rewrite /ir_dis in H. ssa.
+  move: H0 H1 H2 H3 H4 H5 H6 H7.
+  move: v=> [[cur prev]] [re_sch] [[def_pending def_mask]] [[disk_pending disk_mask]] [timer_pending timer_mask].
+  move: v'=> [[cur' prev']] [re_sch'] [[def_pending' def_mask']] [[disk_pending' disk_mask']] [timer_pending' timer_mask'].
+  rewrite /get_ic /update_ic /get_bool_state /update_bool_state /get_I_mask /get_mask' /update_I_pending /update_I_bits /update_I_bits' !pair_rewr.
+  move=> H0 H1 H2 H3 H4 H5 H6 H7.
+  rewrite /get_ic /update_ic /get_bool_state /update_bool_state /get_I_mask /get_mask' /update_I_pending /update_I_bits /update_I_bits' !pair_rewr.    
+  destruct i0.
 
-  eapply map_NI.
-
-  4: eapply maybe_NI.
-  mrw. intros. destruct i. destruct i'.
+  apply/rel_eqpair2;con;first ssa.
+  apply/rel_eqpair2;con;first ssa.
+  apply/rel_eqpair2;con;first ssa.
+  rewrite !pair_rewr.  
+  apply/rel_eqpair2;con. rewrite !pair_rewr.
+  apply/rel_eqpair2;con. eauto.
+  rewrite !pair_rewr. eauto.
   rewrite !pair_rewr.
-  apply rel_eqpair_R2' in H.
-  destruct H. destruct H.
-  apply test_test in H0 as H0'.
-  destruct H0'. destruct i0. destruct i2. ssa. ssa. ssa.
-  destruct i0. ssa. destruct i2. ssa.
-  apply rel_eqmaybe_false2.
-  instantiate (1:= eqpair _ _).
-  apply rel_eqpair2. rewrite !pair_rewr. con.
-  instantiate (1:= publicRel _). (*changed from private to public*)
-  clear H0 H1. Print stateType.
+  apply/rel_eqpair2;con;eauto.
 
-  destruct (eqVneq l \bot). subst. eauto.
-  apply semiprivate_not_bot' in H. subst. eauto. apply/eqP. done.
-  instantiate (1:= eqpair _ _).
-  apply rel_eqpair2. rewrite !pair_rewr. con.
-  instantiate (1:= eqmaybe_top (semiprivateRel _)).
-  apply rel_eqsum_L2' in H0.
-  clear H1.
-  destruct (eqVneq l \bot). subst. apply eqmaybe_semiprivate_bot.
-
-  apply  out_rel_not_bot in H0. subst. eauto. apply/eqP. done.
-  clear H.
-  apply rel_eqsum_L2' in H0.
-  destruct (eqVneq l \bot). subst. eauto.
-  apply  out_rel_not_bot in H0. subst. eauto. apply/eqP. done.
-  destruct H. destruct i0. 2:ssa. destruct i2. 2:ssa. auto.
-  mrw. intros.
-  destruct i.
-  apply dis_eqpair_R in H. destruct i0. 2:ssa.
-  have: dis in_rel l i0. ssa. clear H=>H.
-  rewrite !pair_rewr. done.
-  mrw. intros.
-  apply rel_eqsum_L2. eauto.
-
-  apply par_NI.
-
-  eapply map_NI. 
-  4: eapply swi_NI.
-  mrw. intros.
-  move/rel_eqpair : H. case=>H0 H1.
-  apply rel_eqpair_LR2. con.
-  instantiate (1:= falseRel).
-  
-
-
-  5: { intros. left. apply falseRel_aware. move: H0. clear. ssa. de H0.
-  5: eapply maybe_NI. eauto.
-  2: { mrw. intros. move: H. instantiate (1:= publicRel _). simpl. de i. de i'. de i'. }
-  mrw. ssa. 
-
-  3: { mrw. intros. simpl in i,i'.
-       move: H. instantiate (1:= publicRel _). instantiate (1:= publicRel _). ssa. de i. de i'. de i'. }
-  mrw. intros.
-
-
-  mrw. intros.
-  destruct i. destruct i0.  destruct i'. destruct i3.
+  apply/rel_eqpair2;con;first ssa.
+  apply/rel_eqpair2;con;first ssa.
+  apply/rel_eqpair2;con;first ssa.
+  rewrite !pair_rewr.  
+  apply/rel_eqpair2;con. rewrite !pair_rewr.
+  apply/rel_eqpair2;con. eauto.
+  rewrite !pair_rewr. eauto.
   rewrite !pair_rewr.
-  move:H. move/rel_eqpair=>[] H0 /rel_eqpair [] H1.
-  rewrite !pair_rewr in H0 H1. rewrite !pair_rewr.
-  intros.
-  instantiate (1:= eqpair _ _). apply rel_eqpair2.
-  rewrite !pair_rewr. con.
-  instantiate (1:= semiprivateRel _). move: H0. clear.
-  intros. ssa. de H0. eauto. 2:eauto.
-  mrw. intros. ssa.
+  apply/rel_eqpair2;con;eauto.
 
-  eapply swi_NI.
+  apply/rel_eqpair2;con;first ssa.
+  apply/rel_eqpair2;con;first ssa.
+  rewrite !pair_rewr.    
+  apply/rel_eqpair2;con.
+  apply/rel_eqpair2;con. eauto.
+  rewrite !pair_rewr. eauto.
+  apply/rel_eqpair2;con. rewrite !pair_rewr.
+  apply/rel_eqpair2;con. eauto.
+  rewrite !pair_rewr. eauto.
+  apply/rel_eqpair2;con;eauto.  
+
+
+  destruct i. exfalso;ssa.
+  destruct i'. exfalso;ssa.
+  apply rel_eqsum_L2' in H.
+  clear H1. move: H0.
+  move/rel_eqpair=>[H0] /rel_eqpair[H1] /rel_eqpair[]/rel_eqpair[H2 H3] /rel_eqpair[]/rel_eqpair[H4 H5] /rel_eqpair[] H6 H7.
+  move: H0 H1 H2 H3 H4 H5 H6 H7.
+  move: v=> [[cur prev]] [re_sch] [[def_pending def_mask]] [[disk_pending disk_mask]] [timer_pending timer_mask].
+  move: v'=> [[cur' prev']] [re_sch'] [[def_pending' def_mask']] [[disk_pending' disk_mask']] [timer_pending' timer_mask'].
+  rewrite !pair_rewr.
+  move=> H0 H1 H2 H3 H4 H5 H6 H7.
   
+  rewrite /state_step /step_on_output.
+
+ have: rel stateType_rel l
+    ((inspect_output good_to_bs i)
+       (cur, prev, (re_sch, (def_pending, def_mask, (disk_pending, disk_mask, (timer_pending, timer_mask))))))
+    ((inspect_output good_to_bs i0)
+       (cur', prev', (re_sch', (def_pending', def_mask', (disk_pending', disk_mask', (timer_pending', timer_mask')))))).
+
+ rewrite /inspect_output.
+
+ have:   rel stateType_rel l
+    ((check_scheduler i)
+       (cur, prev, (re_sch, (def_pending, def_mask, (disk_pending, disk_mask, (timer_pending, timer_mask))))))
+    (( check_scheduler i0)
+       (cur', prev', (re_sch', (def_pending', def_mask', (disk_pending', disk_mask', (timer_pending', timer_mask')))))).
+
+ have: is_sch_out i = is_sch_out i0. 
+ move: H=> /rel_eqpair[] + /rel_eqpair[] + /rel_eqpair[] + /rel_eqpair[] _ /rel_eqpair[] _ _.
+ move: i=>[a[] b[] c[] d[] e f].
+ move: i0=>[a'[] b'[] c'[] d'[] e' f']. 
+ rewrite !pair_rewr /is_sch_out.
+ 
+ case/rel_eqmaybe2.
+ move=>[]x []y []-> []->//.
+ case=>->->.
+
+ case/rel_eqmaybe2.
+ move=>[]x []y []-> []->//.
+ case=>->->.
+
+ case/rel_eqmaybe2.
+ move=>[]x []y []-> []->//.
+ move=>/=->//.
+ case=>->->//.
+
+ rewrite /check_scheduler=>->.
+ destruct (is_sch_out i0) eqn:Heqn.
+
+  apply/rel_eqpair2;con;first ssa.
+  apply/rel_eqpair2;con;first ssa.
+  rewrite !pair_rewr.    
+  apply/rel_eqpair2;con;first ssa.
+  apply/rel_eqpair2;con;first ssa.
+  apply/rel_eqpair2;con;first ssa.
+  rewrite !pair_rewr. eauto.
+  apply/rel_eqpair2;con;first ssa.
+  apply/rel_eqpair2;con;first ssa.
+  rewrite !pair_rewr.    
+  apply/rel_eqpair2;con;first ssa.
+  apply/rel_eqpair2;con;first ssa.
+  apply/rel_eqpair2;con;first ssa.  
+  rewrite !pair_rewr. eauto.
+
   
+
+
+ 
+ rewrite /is_I_out_done. rewrite /tI_out. simpl.
+ case: f=>a0.
+ case: f'=>a1. move=>->//. ssa.
+ case: f' a0=>//. ssa.
+ move=> HtI_out.
+
+ 
+ have: tI_out i = tI_out i0.
+ move: H=> /rel_eqpair[] _ /rel_eqpair[] _ /rel_eqpair[] _ /rel_eqpair[] _ /rel_eqpair[] _.
+ move: i=>[a[] b[] c[] d[] e f].
+ move: i0=>[a'[] b'[] c'[] d'[] e' f']. 
+ rewrite !pair_rewr.
+ rewrite /is_I_out_done. rewrite /tI_out. simpl.
+ case: f=>a0.
+ case: f'=>a1. move=>->//. ssa.
+ case: f' a0=>//. ssa.
+ move=> HtI_out.
+
+ rewrite /inspect_output.
+ 
+ move/rel_eqmaybe2.
+ case.
+ move=>[] [h0 b0] [][h1 b1][]->[]->/=[]->->.
+ case: h1.
+ move=>HH.
+ apply rel_eqmaybe2 in HH.
+ Search _ (rel (eqmaybe _)).
+ have: rel (publicRel (Times THandlerOutput Bool)) l f f'. ssa.
+ clear HH => HH.
+ move: f f' HH=> [f b0] [f' b0']=>/=.
+ case=>->->.
+ case: f'.
+
+ rewrite /inspect_output /check_handlers /check_scheduler.
+ rewrite /is_I_out_done.
+
+
+  
+  rew
+  ssa. de v. de p. de s. de v'. de p. de s. de H0.
+  rewrite /update_I_bits'.
+  rewrite !pair_rewr.  
+  apply/rel_eqpair2.
+  simpl in H. destruct H. subst. eauto.
+  have: state_step good_to_bs (inl i) = state_step good_to_bs (inl i). simpl. rewrite /state_step.
   Search _ (rel (eqsum_L _ _)).
-  clear H1.
-
-  apply rel_eqsum_L2' in H0.
-  destruct (eqVneq l \bot). subst.
-  apply eqmaybe_semiprivate_bot.
-  apply semiprivate_not_bot' in H;eauto. subst.
-  apply eqmaybe_semiprivate_not_bot.  
-  ssa.
-  de i0.
-  ssa. de H. subst.
-  Search _ (eqmaybe_false). (Some _)).
-  Search _ (rel (eqpair_R _ _)).  
-  4: eapply par_NI.
-
-
-Lemma model_good_NI : NI in_rel out_rel model_good.
-Proof.
-  rewr;simpl;rewr;simpl.
-  eapply map_NI.
-  instantiate (1:= eqsum_L in_rel out_rel). ssa. ssa.
-  mrw. intros.
-  2:eapply loop_NI. apply test_test in H as H'. destruct H'.
-  destruct i. destruct i'. ssa. ssa. ssa.
-  destruct i. ssa. destruct i'. ssa.
-  apply rel_eqsum_L2' in H. 
-  rewrite /inr_or_def. done.
-
-  eapply map_NI.
-  eauto. eauto.
-  mrw. intros.
-  2:apply sta_NI. apply rel_eqpair in H. destruct H. eauto.
-  instantiate (1:= semiprivateRel _). ssa. mrw. intros.
-  simpl in H0. subst.
-  destruct H0. destruct H0. subst.
-  apply test_test in H as H'.
-  destruct H'. destruct i. destruct i'. ssa.
   destruct i. destruct i0. destruct H. subst. ssa. ssa.
   left. ssa.
   move: H H3. rewrite /ir_dis. ssa. done. de i0. done. ssa.
@@ -1014,6 +1207,17 @@ Proof.
   apply out_rel_not_bot in H. subst. eauto. done.
   subst. eauto.
 
+
+
+
+
+
+
+
+
+
+  
+
   mrw. intros. destruct i. 2:ssa.
   have: dis in_rel l i. ssa. clear H=>H.
   destruct (eqVneq l \bot). subst. ssa.
@@ -1108,3 +1312,4 @@ Proof.
   Search _ (eqmaybe_false). (Some _)).
   Search _ (rel (eqpair_R _ _)).  
   4: eapply par_NI.
+
